pretty much admit free

proof/correctness/avx2/MLKEM_InnerPKE_avx2.ec
@@ -1856,7 +1856,6 @@ qed.
 *)
 bind op [W16.t & W256.t & Array256.t] sliceget256_16_256 "asliceget".
 realize bvaslicegetP.
-
 move => /= arr offset; rewrite /sliceget256_16_256 /= => H k kb. 
 case (8%| offset) => /= *; last by smt(W256.get_bits2w).
 rewrite /get256_direct pack32E initiE 1:/# /= initiE 1:/# /= initiE 1:/# /= bits8E initiE 1:/# /=.
@@ -1973,31 +1972,119 @@ rewrite (nth_map W16.zero []); 1: smt(Array256.size_to_list).
 rewrite nth_mkseq 1:/# /= bits8E /= initiE /# /=.
 qed.
 
-op sliceget32_8_256 (arr: W8.t Array32.t) (i: int) : W256.t = get256 (WArray32.init8 (fun (i_0 : int) => pvc_shufbidx_s.[i_0])) (i%/256).
+op sliceget32_8_256 (arr: W8.t Array32.t) (offset: int) : W256.t = 
+if 8 %| offset then 
+    get256_direct (WArray32.init8 (fun (i_0 : int) => arr.[i_0])) (offset %/ 8)
+   else W256.bits2w (take 256 (drop offset (flatten (map W8.w2bits (to_list arr))))).
 
 bind op [W8.t & W256.t & Array32.t] sliceget32_8_256 "asliceget".
-realize bvaslicegetP by admit.  (* We need a general framework for these *)
+realize bvaslicegetP.
+move => /= arr offset; rewrite /sliceget32_8_256 /= => H k kb. 
+case (8%| offset) => /= *; last by smt(W256.get_bits2w).
+rewrite /get256_direct pack32E initiE 1:/# /= initiE 1:/# /= initiE 1:/# /=. 
+rewrite nth_take 1,2:/# nth_drop 1,2:/#.
+rewrite (BitEncoding.BitChunking.nth_flatten false 8 _). 
++ rewrite allP => x /=; rewrite mapP => He; elim He;smt(W8.size_w2bits).
+rewrite (nth_map W8.zero []); 1: smt(Array32.size_to_list).
+by rewrite nth_mkseq /#.
+qed.
 
-op sliceget768_16_256 (arr: W16.t Array768.t) (i: int) : W256.t = get256 (WArray1536.init16 (fun (i_0 : int) => arr.[i_0])) (i %/ 256). 
+op sliceget768_16_256 (arr: W16.t Array768.t) (offset: int) : W256.t =
+if 8 %| offset then 
+    get256_direct (WArray1536.init16 (fun (i_0 : int) => arr.[i_0])) (offset %/ 8)
+   else W256.bits2w (take 256 (drop offset (flatten (map W16.w2bits (to_list arr))))).
+
 
 bind op [W16.t & W256.t & Array768.t] sliceget768_16_256 "asliceget".
-realize bvaslicegetP by admit.  (* We need a general framework for these *)
+realize bvaslicegetP.
+move => /= arr offset; rewrite /sliceget768_16_256 /= => H k kb. 
+case (8%| offset) => /= *; last by smt(W256.get_bits2w).
+rewrite /get256_direct pack32E initiE 1:/# /= initiE 1:/# /= initiE 1:/# /= bits8E initiE 1:/# /=.
+rewrite nth_take 1,2:/# nth_drop 1,2:/#.
+rewrite (BitEncoding.BitChunking.nth_flatten false 16 _). 
++ rewrite allP => x /=; rewrite mapP => He; elim He;smt(W16.size_w2bits).
+rewrite (nth_map W16.zero []); 1: smt(Array768.size_to_list).
+by rewrite nth_mkseq /#.
+qed.
 
-op sliceset960_8_128 (arr: W8.t Array960.t) (i: int) (bv: W128.t) : W8.t Array960.t = Array960.init (get8 (set128_direct ((init8 (fun (i_0 : int) => arr.[i_0])))%WArray960 (i %/ 8) bv)).
+op sliceset960_8_128 (arr: W8.t Array960.t) (offset: int) (bv: W128.t) : W8.t Array960.t = 
+  if 8 %| offset
+  then Array960.init (fun (i3 : int) => get8 (set128_direct ((init8 (fun (i_0 : int) => arr.[i_0])))%WArray960 (offset %/ 8) bv) i3)
+  else  Array960.of_list witness (map W8.bits2w (chunk 8 (take offset (flatten (map W8.w2bits (to_list arr))) ++ w2bits bv ++
+  drop (offset + 128) (flatten (map W8.w2bits (to_list arr)))))).
+
+lemma size_flatten_W8_w2bits (a : W8.t list) :
+  (size (flatten (map W8.w2bits (a))))  =  8 * size a.
+proof.
+  rewrite size_flatten -map_comp /(\o) /=.
+  rewrite StdBigop.Bigint.sumzE /= StdBigop.Bigint.BIA.big_mapT /(\o) /=. 
+  rewrite StdBigop.Bigint.big_constz count_predT /#.
+qed.
 
 bind op [W8.t & W128.t & Array960.t] sliceset960_8_128 "asliceset".
-realize bvaslicesetP by admit.  (* We need a general framework for these *)
+realize bvaslicesetP.
+move => arr offset bv H /= k kb; rewrite /sliceset960_8_128 /=. 
+case (8 %| offset) => /= *; last first.
++ rewrite of_listK; 1: by  rewrite size_map size_chunk // !size_cat size_take; 
+      by smt(size_take size_drop  W8.size_w2bits size_cat Array960.size_to_list size_flatten_W8_w2bits size_ge0). 
+  rewrite -(map_comp W8.w2bits W8.bits2w) /(\o). 
+  have := eq_in_map ((fun (x : bool list) => w2bits ((bits2w x))%W8)) idfun (chunk 8
+        (take offset (flatten (map W8.w2bits (to_list arr))) ++ w2bits bv ++
+         drop (offset + 128) (flatten (map W8.w2bits (to_list arr))))).
+  rewrite iffE => [#] -> * /=; 1: by smt(in_chunk_size W8.bits2wK).
+  rewrite map_id /= chunkK //;1: by rewrite !size_cat size_take;
+    by smt(size_take size_drop  W8.size_w2bits size_cat Array960.size_to_list size_flatten_W8_w2bits size_ge0). 
+  by rewrite !nth_cat !size_cat /=;
+     smt(nth_take nth_drop size_take size_drop  W8.size_w2bits size_cat Array960.size_to_list size_flatten_W8_w2bits size_ge0). 
+rewrite (nth_flatten _ 8); 1: by rewrite allP => i;rewrite mapP => He; elim He;smt(W8.size_w2bits).
+rewrite (nth_map W8.zero []); 1: smt(Array960.size_to_list).
+rewrite nth_mkseq 1:/# /= initiE 1:/# /= /get8 /set128_direct.
+rewrite initiE 1:/# /=.
+case (offset <= k && k < offset + 128) => *; 1: by 
+  rewrite ifT 1:/#  get_bits8 /= 1,2:/# initiE // initiE //.
+rewrite ifF 1:/# initiE 1:/# /=.
+rewrite (nth_flatten _ 8); 1: by rewrite allP => i;rewrite mapP => He; elim He;smt(W8.size_w2bits).
+rewrite (nth_map W8.zero []); 1: smt(Array960.size_to_list).
+rewrite nth_mkseq /#.
+qed.
 
 
-op sliceset960_8_32 (arr: W8.t Array960.t) (i: int) (bv: W32.t) : W8.t Array960.t = Array960.init
+op sliceset960_8_32 (arr: W8.t Array960.t) (offset: int) (bv: W32.t) : W8.t Array960.t = 
+  if 8 %| offset
+  then Array960.init
      (WArray960.get8
         (set32_direct (WArray960.init8 (fun (i_0 : int) => arr.[i_0])) (
-           i %/ 8) bv)).
+           offset %/ 8) bv))
+  else  Array960.of_list witness (map W8.bits2w (chunk 8 (take offset (flatten (map W8.w2bits (to_list arr))) ++ w2bits bv ++
+  drop (offset + 32) (flatten (map W8.w2bits (to_list arr)))))).
 
 
 bind op [W8.t & W32.t & Array960.t] sliceset960_8_32 "asliceset".
-realize bvaslicesetP by admit.  (* We need a general framework for these *)
-
+realize bvaslicesetP.
+move => arr offset bv H /= k kb; rewrite /sliceset960_8_32 /=. 
+case (8 %| offset) => /= *; last first.
++ rewrite of_listK; 1: by  rewrite size_map size_chunk // !size_cat size_take; 
+      by smt(size_take size_drop  W8.size_w2bits size_cat Array960.size_to_list size_flatten_W8_w2bits size_ge0). 
+  rewrite -(map_comp W8.w2bits W8.bits2w) /(\o). 
+  have := eq_in_map ((fun (x : bool list) => w2bits ((bits2w x))%W8)) idfun (chunk 8
+        (take offset (flatten (map W8.w2bits (to_list arr))) ++ w2bits bv ++
+         drop (offset + 32) (flatten (map W8.w2bits (to_list arr))))).
+  rewrite iffE => [#] -> * /=; 1: by smt(in_chunk_size W8.bits2wK).
+  rewrite map_id /= chunkK //;1: by rewrite !size_cat size_take;
+    by smt(size_take size_drop  W8.size_w2bits size_cat Array960.size_to_list size_flatten_W8_w2bits size_ge0). 
+  by rewrite !nth_cat !size_cat /=;
+     smt(nth_take nth_drop size_take size_drop  W8.size_w2bits size_cat Array960.size_to_list size_flatten_W8_w2bits size_ge0). 
+rewrite (nth_flatten _ 8); 1: by rewrite allP => i;rewrite mapP => He; elim He;smt(W8.size_w2bits).
+rewrite (nth_map W8.zero []); 1: smt(Array960.size_to_list).
+rewrite nth_mkseq 1:/# /= initiE 1:/# /= /get8 /set32_direct.
+rewrite initiE 1:/# /=.
+case (offset <= k && k < offset + 32) => *; 1: by 
+  rewrite ifT 1:/#  get_bits8 /= 1,2:/# initiE // initiE //.
+rewrite ifF 1:/# initiE 1:/# /=.
+rewrite (nth_flatten _ 8); 1: by rewrite allP => i;rewrite mapP => He; elim He;smt(W8.size_w2bits).
+rewrite (nth_map W8.zero []); 1: smt(Array960.size_to_list).
+rewrite nth_mkseq /#.
+qed.
 
 theory W10.
 abbrev [-printing] size = 10.
@@ -2099,17 +2186,19 @@ qed.
 
 
 op sll_64 (w1 w2 : W64.t) : W64.t =
-  if (to_uint w2 < 64) then w1 `<<` (truncateu8 w2) else W64.zero.
+  if (64 <= to_uint w2) then W64.zero else w1 `<<` (truncateu8 w2).
 
 bind op [W64.t] sll_64 "shl".
 realize bvshlP. 
 proof.
 rewrite /sll_64 => bv1 bv2.
-case : (to_uint bv2 < 64).
+case : (64 <= to_uint bv2); last first.
 + rewrite /(`<<`) W64.to_uint_shl; 1: by smt(W8.to_uint_cmp).
   rewrite /truncateu8  => bv2bnd />.
   do 2! (rewrite (pmod_small (to_uint bv2) _);smt(W64.to_uint_cmp)).
-admit. (* What is the circuit behavior? Does it give zero? Yes. *) 
+move => *. 
+have -> : to_uint bv2 = (to_uint bv2 - 64) + 64 by ring. 
+by rewrite exprD_nneg 1,2:/# /= /#.
 qed.
 
 bind op [W32.t & W16.t] W2u16.truncateu16 "truncate".
@@ -2199,16 +2288,29 @@ qed.
 
 
 op sra_32 (w1 w2 : W32.t) : W32.t =
-  w1 `|>>` (truncateu8 w2).
+  if (32 <= to_uint w2) then W32.zero else w1 `|>>` (truncateu8 w2).
 
 bind op [W32.t] sra_32 "ashr".
-realize bvashrP by admit.
+realize bvashrP.
+rewrite /sra_32 => bv1 bv2.
+case : (32 <= to_uint bv2 < 32); last by admit.
+move => *. 
+have -> : to_uint bv2 = (to_uint bv2 - 32) + 32 by ring. 
+rewrite exprD_nneg 1,2:/# /= mulrC. by admit. 
+qed.
 
 op sra_16 (w1 w2 : W16.t) : W16.t =
-  w1 `|>>` (truncateu8 w2).
+if (16 <= to_uint w2) then  W16.zero else w1 `|>>` (truncateu8 w2).
 
 bind op [W16.t] sra_16 "ashr".
-realize bvashrP by admit.
+realize bvashrP.
+rewrite /sra_16 => bv1 bv2.
+case : (16 <= to_uint bv2); last by admit.
+move => *. 
+have -> : to_uint bv2 = (to_uint bv2 - 16) + 16 by ring. 
+rewrite exprD_nneg 1,2:/# /= mulrC. by admit. 
+qed.
+
 
 op srl_16 (w1 w2 : W16.t) : W16.t =
   if 16 <= (to_uint w2) then W16.zero else
@@ -2216,48 +2318,48 @@ op srl_16 (w1 w2 : W16.t) : W16.t =
 
 bind op [W16.t] srl_16 "shr".
 realize bvshrP.
-move => w1 w2. 
-rewrite /srl_16.
-case : (16 <= to_uint w2).
-move => gt.
-simplify.
-rewrite eq_sym.
-apply (divz_eq0 (to_uint w1) (2 ^ to_uint w2)). 
-smt(StdOrder.IntOrder.expr_gt0).
-split.
-smt(W16.to_uint_cmp).
-have : (2 ^ 16 <= 2 ^ (to_uint w2)).
-apply StdOrder.IntOrder.ler_weexpn2l => //. 
-
-move => bnd2.
-smt(W16.to_uint_cmp).
-move => bnd.
-have : (to_uint w2 < 16).
-smt().
-move => bnd2.
-
-rewrite /srl_16 /(`>>`) to_uint_shr.
-smt(W16.to_uint_cmp).
-rewrite /truncateu8.
-rewrite to_uint_small.
-smt(W16.to_uint_cmp).
-congr. congr.
-rewrite pmod_small.
-smt(W16.to_uint_cmp).
-trivial.
+rewrite /srl_16 => bv1 bv2.
+case : (16 <= to_uint bv2); last first.
++ rewrite /(`>>`) W16.to_uint_shr; 1: by smt(W8.to_uint_cmp).
+  rewrite /truncateu8  => bv2bnd />.
+  do 2! (rewrite (pmod_small (to_uint bv2) _);smt(W16.to_uint_cmp)).
+move => *. 
+have -> : to_uint bv2 = (to_uint bv2 - 16) + 16 by ring. 
+rewrite exprD_nneg 1,2:/# /=. 
+smt(StdOrder.IntOrder.expr_gt0 W16.to_uint_cmp pow2_16).
 qed.
 
+
 op sll_16 (w1 w2 : W16.t) : W16.t =
-  w1 `<<` (truncateu8 w2).
+  if (16 <= to_uint w2) then  W16.zero else  w1 `<<` (truncateu8 w2).
 
 bind op [W16.t] sll_16 "shl".
-realize bvshlP by admit. (* not provable. missing %% 65536? *)
+realize bvshlP.
+rewrite /sll_16 => bv1 bv2.
+case : (16 <= to_uint bv2); last first.
++ rewrite /(`<<`) W16.to_uint_shl; 1: by smt(W8.to_uint_cmp).
+  rewrite /truncateu8  => bv2bnd />.
+  do 2! (rewrite (pmod_small (to_uint bv2) _);smt(W16.to_uint_cmp pow2_16)).
+move => *. 
+have -> : to_uint bv2 = (to_uint bv2 - 16) + 16 by ring. 
+by rewrite exprD_nneg 1,2:/# /= /#.
+qed.
 
 op srl_64 (w1 w2 : W64.t) : W64.t =
-  w1 `>>` (truncateu8 w2).
+  if (64 <= to_uint w2) then  W64.zero else  w1 `>>` (truncateu8 w2).
 
 bind op [W64.t] srl_64 "shr".
-realize bvshrP by admit.  (* not provable. missing %% 256? *)
+realize bvshrP.
+rewrite /srl_64 => bv1 bv2.
+case : (64 <= to_uint bv2); last first.
++ rewrite /(`>>`) W64.to_uint_shr; 1: by smt(W8.to_uint_cmp).
+  rewrite /truncateu8  => bv2bnd />.
+  do 2! (rewrite (pmod_small (to_uint bv2) _);smt(W64.to_uint_cmp)).
+move => *. 
+have -> : to_uint bv2 = (to_uint bv2 - 64) + 64 by ring. 
+rewrite exprD_nneg 1,2:/# /=. 
+smt(StdOrder.IntOrder.expr_gt0 W64.to_uint_cmp pow2_64).
+qed.
 
 op lane_func_reduce(c : W16.t) : W16.t =  
     let t =  (sigextu32 c)  * (W32.of_int 20159) in
